|Правило Бернулли-Лопиталя: $f(x)$ и $g(x)$ дифференцируемы на $(a,b), \ \ g'(x)\neq0$
1. $f(x)\longrightarrow 0, \ g(x)\longrightarrow 0 \ \ x\longrightarrow b-0$
2. $g(x)\longrightarrow\infty$ при $x\longrightarrow b-0$
Тогда, если $\exists \lim_{ x \to b-0 } \frac{f'(x)}{g'(x)}\implies \exists \lim_{ x \to b-0 } \frac{f(x)}{g(x)}$ и $\lim_{ x \to b-0 } \frac{f'(x)}{g'(x)} =\lim_{ x \to b-0 } \frac{f(x)}{g(x)}$

$$\frac{f(x)}{g(x)}= \frac{f(x)-f(a)(=0)}{g(x)-g(a)(=0)}=\frac{f(x)-f(a)}{x-a}: \frac{x-a}{g(x)-g(a)}= \frac{ \frac{f(x)-f(a)}{x-a} }{\frac{g(x)-g(a)}{x-a}} \longrightarrow_{x\longrightarrow 0} \frac{f'(x)}{g'(x)}$$
![[Pasted image 20241226194235.png]]
*Док-во:* (теорема Коши о конечных приращениях)
$A:=\lim_{ x \to b-0 } \frac{f'(x)}{g'(x)}, b \in \mathbb{R}\quad \ f(b):=0 \ \ g(b):=0$
1. $\frac{f(x)}{g(x)}=\frac{f(x)-f(b)}{g(x)-g(b)}= \frac{f'(\xi)}{g'(\xi)} \longrightarrow_{x\longrightarrow b-0} A \quad \xi \in(x,b)$ 
![[Pasted image 20241226194537.png]]
2. $\forall x,y\in(a,b)$
	![[Pasted image 20241226194714.png]]
	$\frac{f(x)-f(y)}{g(x)-g(y)}= \frac{f'(\xi)}{g'(\xi)} \ \ \exists \xi \in(y,x)$
	$$f(x)= \frac{f'(\xi))}{g'(\xi)}(g(x)+g(y))+f(y) \ \ \ \frac{f(x)}{g(x)}= \frac{f'(\xi)}{g'(\xi)}\left( 1- \frac{g(y)}{g(x)} \right) + \frac{f(y)}{g(x)}$$
$$| \frac{f(x)}{g(x)}-A| \trianglelefteq | \frac{f'(\xi)}{g'(\xi)}-A|+ |  \frac{f'(\xi)}{g'(\xi)} \frac{g(y)}{g(x)}|+ | \frac{f(y)}{g(x)}|$$
$$\forall\varepsilon>0 \ \exists\delta>0:\forall t\in(b-\delta ,b) \ \ \ | \frac{f'(t)}{g'(t)}-A|< \frac{\varepsilon}{3}+ \text{отсюда же(?)}$$
$\frac{f'(t)}{g'(t)}$ в $(b-\delta,b) \ \ \forall x\in(y,b) \ \ \forall y\in(b-\delta,b)$, т.к. $\xi \in(y,b)\implies$
$$| \frac{f'(\xi)}{g'(\xi)} \frac{g(y)(=const)}{g(x)(\longrightarrow \infty)}| \longrightarrow_{x\longrightarrow b- 0} 0\quad | \frac{f(y)}{f(x)}|\longrightarrow_{x\longrightarrow b-0} 0\implies \delta'=\delta_{y,b}>0: \ \forall x \in(b-\delta',b)$$
$$| \frac{f'(\xi)}{g'(\xi)} \frac{g(y)}{g(x)}|< \frac{\varepsilon}{3} \ \ \ | \frac{f(y)}{g(x)}|< \frac{\varepsilon}{3} \ \ \ | \frac{f(x)}{g(x) } -A|< \frac{\varepsilon}{3}+ \frac{\varepsilon}{3} + \frac{\varepsilon}{3} = \varepsilon$$
$b=+\infty \quad x\longrightarrow+\infty \ \ t= \frac{1}{x}\longrightarrow +0 \ \ t\longrightarrow+0$
$\phi(t):=f\left( \frac{1}{t} \right)$ 
$\psi(t):=g\left( \frac{1}{t} \right)$
$$\lim_{ x \to +\infty } \frac{f(x)}{g(x)}= \lim_{ t \to +0 } \frac{f\left( \frac{1}{t} \right)}{g\left( \frac{1}{t} \right)}=\lim_{ t \to +0 } \frac{\phi(t)}{\psi(t)}= \lim_{ t \to +0 } \frac{\phi'(t)}{\psi'(t)}=\lim_{ t \to +0 } \frac{  f'\left( \frac{1}{t} \right) \left( -\frac{1}{t^{2}} \right) }{g'\left( \frac{1}{t} \right) \left( -\frac{1}{t^{2}} \right)}=\lim_{ x \to +\infty } \frac{f'(x)}{g'(x)}$$

Замечание. $\lim_{ x \to +\infty } \frac{\log x}{x^{\xi}}=\lim_{ x \to +\infty } \frac{ \frac{1}{x} }{\varepsilon x^{\varepsilon-1}}=\lim_{ x \to +\infty } \frac{1}{\varepsilon x^{\varepsilon}}=0$
$\frac{x^{\alpha}}{a^{x}},\ x^{2}\log x \ x\longrightarrow+0\quad \lim_{ x \to +\infty } \frac{2x+\sin x}{2x+\cos x}=1 \not= \lim_{ x \to +\infty } \frac{2+\cos x}{2-\sin x}$ не определён
$0,\infty= \frac{0}{\frac{1}{\infty}}=\frac{\infty}{\frac{1}{0}}; \ 1^{\infty}=e^{ \infty \log 1 }\quad 0^{0}=e^{ \log 0 \cdot 0 }\quad \infty^{0}=e^{ \log \infty \cdot_{0} }$
$(+\infty)_{1}-(+\infty)_{2}= \frac{(+\infty)^{2}_{1}-(+\infty)^{2}_{2}}{(+\infty)_{1}+(+\infty)_{2}}\quad \frac{0}{0} \ \ \ \frac{?}{\infty}$


