$x_{0}=0$ 
1. $f(x)=e^{ x }$
	$(e^{ x })^{(k)}=e^{ x }, e^{ 0 }=1 \ \ \ \forall x\in \mathbb{R},\forall n\in \mathbb{N} \ \ \exists\xi=\xi(x,n)\in(0,x)$
	$e^{ x }=\sum_{k=0}^{n} \frac{x^{k}}{k!}+\frac{e^{ \xi }}{(n+1)!}x^{n+1} \ \ n\longrightarrow\infty$
	$|r_{n}(x,x_{0})|=\frac{e^{ \xi }}{(n+1)!}|x|^{n+1}< \frac{e^{ |x| }}{(n+1)!}|x|^{n+1}=e^{ |x| } \frac{|x|^{n+1}}{(n+1)!}\longrightarrow 0, \ \ n\longrightarrow\infty$
	$\frac{|x|^{n+1}}{(n+1)!}= \frac{|x|}{1}\cdot\frac{|x|}{2}\cdot\dots \frac{\cdot|x|}{[|x|]+1}\cdot\dots\cdot \frac{|x|}{n}\cdot \frac{|x|}{n+1}\longrightarrow_{n\longrightarrow\infty} 0\ \ \ \forall x\in \mathbb{R}$ фиксированно
$$e^{ x }=\lim_{ n \to \infty } \sum_{0}^{n} \frac{x^{k}}{k!}=\sum_{0}^{\infty} \frac{x^k}{k!}$$
$e^{ x }=\sum_{0}^{n} \frac{x^{k}}{k!}+ o(x^{n}) \ \ n\longrightarrow \infty$ Пеано
				$O(x^{n+1})$ Лагранж
$e=e^{1}=\sum_{0}^{\infty} \frac{1}{k!}\quad e-\sum_{0}^{\infty} \frac{1}{k!}= \frac{e^{ \xi_{n} }}{(n+1)!}< \frac{e}{(n+1)!}\quad \exists\xi_{n}\in(0,1)$
2. &3 $\sin x$ и $\cos x$
	$\sin'x=\cos x=\sin\left(  \frac{\pi}{2} +x\right)$
	$\sin^{(k)}x=\sin \left( x+k\cdot \frac{\pi}{2} \right), \quad \cos^{(k)}x=\cos\left( x+k\cdot \frac{\pi}{2} \right)$
	$$\sin^{(k)}(0)=\sin \frac{\pi k}{2} = \begin{cases}
0\quad k=2m \\
(-1)^{m} \quad k=2m+1
\end{cases}$$
$$\cos^{(k)}(0)=\cos \frac{\pi k}{2}= \begin{cases}
(-1)^{m}\quad k=2m \\
0\quad k=2m+1
\end{cases}$$
$\sin x=\sum_{k=0}^{n} \frac{(-1)^{k}}{(2k+1)!}x^{2k+1}+r_{2n+1}(x,0)+r_{2n+2}(x,0)\ \ \ \exists\xi \in(0,x)$
$$r_{2n+2}(x,0)= \frac{\sin^{2n+3}\xi}{(2n+3)!}x^{2n+3}=\sin\left( \xi+ \frac{(2n+3)\pi}{2} \right)(\text{ограничена}) \frac{x^{2n+3}}{(2n+3)!(n\longrightarrow\infty)}\longrightarrow_{n\longrightarrow\infty} 0$$
$$\sin x=\sum_{k=0}^{n} \frac{(-1)^k}{(2k+1)!}x^{2n+1}$$
$\sin x=\sum_{k=0}^{n} \frac{(-1)^k}{(2k+1)!}x^{2n+1}+o(x^{2n+1})+O(x^{2n+2})$
Аналогично
$$\cos x=\sum_{k=0}^{n} \frac{(-1)^{k}}{(2k)!}x^{2k}$$
$\cos x=\sum_{k=0}^{n} \frac{(-1)^{k}}{(2k)!}x^{2k}+o(x^{2n}+O(x^{2n+1})) \ \ \ x\longrightarrow 0$
$e^{ x }=\sum_{0}^{\infty} \frac{x^{k}{k!}}\ \ \forall x \ \ e^{ x }:=\sum_{0}^{\infty} \frac{x^{k}}{k!} \ \ \ \ e^{ z_{1}+z_{2} }=e^{ z_{1} }e^{ z_{2} }\quad e^{ iz }=\sum_{0}^{\infty} \frac{(iz)^{k}}{k!}=\cos z+i\sin z  \ \ (e^{ z }\neq 0 \ \ \forall z)$
4. $f(x)=\log(1+x)$
	$\log'(x+1)= \frac{1}{1+x}= (1+x)^{-1},$ при $k\geq 2$
	$\log^{(k)}(1+x)=((1+x)^{-1})^{(k-1)}=(-1)(-2)\cdot\dots \cdot(-(k-1))(1+x)^{-k}= \ \frac{(-1)^{k-1}(k-1)!}{(1+x)^{k}}$
	$\log(1+x)=\sum_{k=1}^{n} \frac{\log^{(k)}(1+x)|_{x=0}}{k!}x^{k}+r_{n}(x,0)=\sum_{k=1}^{n} \frac{(-1)^{k-1}}{k}x^{k}+r_{n}(x,0)$
$$\log(1+x)\thicksim \sum_{k=1}^{\infty} \frac{(-1)^{k-1}x^{k}}{k}\quad |x|<1 \text{ сходится}$$
$$\text{д'Аламбер } | \frac{a_{n+1}}{a_{n}}|=| \frac{\left( \frac{(-1)^{n}x^{n+1}}{n+1} \right)}{\frac{(-1)^{n-1}x^{n}}{n}} |= \frac{n|x|}{x+1}\longrightarrow|x|$$
$$\log'(1+x)= \frac{1}{1+x}=\frac{1}{1-(-x)}=1+(-x)+(-x^{2})+\dots+\dots=1-x+x^{2}-x^{3}+\dots+(-1)^{n}x^{n}+$$
$$\log(1+x)=\sum_{k=1}^{n} \frac{(-1)^{k}x^{k}}{k}+\frac{\log^{(n+1)}(1+x))|_{x=\xi}}{(n+1)!}x^{n+1}=\sum_{k=1}^{n} \frac{(-1)^{k}x^{k}}{k}+ \frac{(-1)^{n}x^{n+1}n!}{(n+1)!(1+\xi)^{n+1}}$$
$$=\sum_{k=1}^{n} \frac{(-1)^{k}x^{k}}{k}+(\frac{(-1)^{n}}{n+1} \ \frac{x^{n+1}}{(1+\xi)^{n+1}})(=r_{n}(x,0))$$
$$|r_{n}(x,0)|= \frac{1}{n+1} | \frac{x}{1+\xi}|^{n+1} \longrightarrow_{n\longrightarrow \infty} 0\quad |x|<1, \ \xi \in(0,x)\ \ \ \xi=\xi(n,x)$$
1. $x>0\implies 0<x<1<1+\xi \ \ (\xi>0)$, если $x>0\implies |\frac{x}{1+\xi}|<1\implies r_{n}(x,0)\longrightarrow 0$
2. $x<0 \ x\in(-1,0) \ \ \xi \in(x,0)$
	$| \frac{x}{1+\xi}|= \frac{|x|}{1-|\xi|}< \frac{|x|}{1-|x|}<1 |x|<1-|x| \ \ |x|< \frac{1}{2} \ \ x\in\left( -\frac{1}{2};1 \right) \ \ x=1? \ \ x\in\left( -1;-\frac{1}{2} \right)?$
5. $f(x)=(1+x)^{\alpha} \ \ \alpha \in \mathbb{R}$
	$f^{(k)}(x)=\alpha(\alpha-1)\dots(\alpha-k+1)(1+x)^{\alpha-k}$
	$f^{(k)}(0)=\alpha(\alpha-1)\dots(\alpha-k+1) \frac{\alpha!}{(\alpha-k)!} \ \ \ \alpha \in \mathbb{N}$
	1. $\alpha \in \mathbb{N} \ \ \ f(x)=(1+x)^{\alpha}=\sum_{k=0}^{\alpha} \frac{1}{k!} \frac{\alpha!}{(\alpha-k)!}x^{k}=\sum_{k=0}^{\alpha}C^{k}_{\alpha}x^{k} \ \ k>\alpha \ \ f^{(k)}(0)=0$
	2. $\alpha \not\in \mathbb{N}$
		$(1+x)^{\alpha}=1+\alpha x+ \frac{\alpha(\alpha-1)}{2!}x^{2}+\dots+ \frac{\alpha(\alpha-1)\dots(\alpha-n+1)}{n!}x^{n}+r_{n}(x,0)+o(x^{n}) \ \ \ x\longrightarrow 0$
д'Аламбер
$$ | \frac{a_{n+1}}{a_{n}}|=|\frac{\alpha(\alpha-1)\dots(\alpha-n+1)(\alpha-n)x^{n+1}}{(n+1)!} \ \frac{n!}{\alpha(\alpha-1)\dots(\alpha-n+1)x^{n}}|=| \frac{\alpha-n}{n+1}||x|\longrightarrow |x|$$
$|x|<1$ сходится
$x\pm 1$ в зависимости от $\alpha$ 
$$(1+x)^{\alpha}=\sum_{0}^{\infty}C^{k}_{\alpha}x^{k}$$
	