---
tags:
  - calculus
  - integral
---

Вид выражений $\int R(x, \sqrt{ ax^{2}+bx+c })dx$
1. Подстановка Эйлера, $a>0$
	$\sqrt{ ax^{2}+bx+c }= t-x\sqrt{ a }\to ax^{2}+bx+c=t^{2}-2tx\sqrt{ a }+x^{2}a\to x(b+2t\sqrt{ a })=t^{2}-c$
$$x= \frac{t^{2}-c}{2t\sqrt{ a }+b}=r(t), \sqrt{ ax^{2}+bx+c }=t-r(t)\sqrt{ a }=r_{1}(t), dx=r_{2}(t)dt$$
	где $r(t),r_{1}(t),r_{2}(t)$ - рациональные функции $t\implies I(t)=\int \tilde{R}(t)dt$
	Пример: $\int \sqrt{ x^{2}+a^{2} }dx$
	$$\sqrt{ x^{2}+a^{2} }=t-x\to x^{2}+a^{2}=t^{2}-2tx+x^{2}\to x= \frac{t^{2}-a^{2}}{2t}, \sqrt{ x^{2}+a^{2} }=t- \frac{t^{2}-a^{2}}{2t}= \frac{t^{2}+a^{2}}{2t}$$
	$$dx= \frac{1}{2} \frac{2t^{2}-(t^{2}-a^{2})}{t^{2}}dt= \frac{t^{2}+a^{2}}{2t^{2}}dt$$
	$$I(t)=\int \frac{(t^{2}+a^{2})^{2}}{2t^{2}\cdot{2}t}= \frac{1}{4}\int \frac{t^{4}+2t^{2}a^{2}+a^{4}}{t^{3}}dt=\frac{1}{4}\int\left( t+\frac{2a^{2}}{t} +\frac{a^{4}}{t^{3}} \right)dt$$
	$$=\frac{1}{4} \frac{t^{2}}{2} + 2a^{2}\ln|t| - \frac{1}{2}\frac{a^{4}}{t^{2}} +\frac{a^{2}}{2}\ln|t|=\frac{1}{8}((x+\sqrt{ x^{2}+a^{2} })^{2}+(x-\sqrt{ x^{2}+a^{2} })^{2}) + $$
$$+\frac{a^{2}}{2}\ln|x+\sqrt{ x^{2}+a^{2} }| +C$$
	$$=\frac{1}{8}4x\sqrt{ x^{2}+a^{2} }+ \frac{a^{2}}{2}\ln|x+\sqrt{ x^{2}+a^{2} }=\frac{1}{2}x\sqrt{ x^{2}+a^{2} } + \frac{a^{2}}{2}\ln|x+\sqrt{ x^{2}+a^{2} }|+C$$
2. Подстановка Эйлера, $c>0$
	$$\sqrt{ ax^{2}+bx+c }=x\cdot t+\sqrt{ c }\implies ax^{2}+bx+c+x^{2}t^{2}+2xt\sqrt{ c }+c\to ax+b=xt^{2}+2t\sqrt{ c }$$
	$$x(t^{2}-a)=b-2t\sqrt{ c }\to x= \frac{b-2t\sqrt{ c }}{t^{2}-a}=r(t), \sqrt{ ax^{2}+bx+c }=t\cdot r(t)+\sqrt{ c }=r_{1}(t), dx=r_{2}(t)dt$$
	$$I(t)=\int \tilde{R}(t)dt$$
	Пример $\int \frac{dx}{x+\sqrt{ x^{2}-x+1 }}, c=1>0$
	$$\sqrt{ x^{2}-x+1 }=xt+1\to x^{2}-x+1=x^{2}t^{2}+2xt+1\to x-1=xt+2t\to$$
	$$x(1-t^{2})=1+2t\to x= - \frac{2t+1}{t^{2}-1}\to x+\sqrt{ x^{2}-x+1 }= - \frac{(2t-1)t}{t^{2}-1} + 1 - \frac{2t+1}{t^{2}-1} =$$
	$$= \frac{-2t^{2}-t+t^{2}-1-2t-1}{t^{2}-1}= \frac{-t^{2}-3t-2}{t^{2}-1};$$
	$$dx=- \frac{2(t^{2}-1) - (2t+1)2t}{(t^{2}-1)^{2}}dt= \frac{-2t^{2}-2t-2}{(t^{2}-1)^{2}}dt= 2 \frac{t^{2}+t+1}{(t^{2}-1)^{2}}dt$$
	$$I(t)= - \int \frac{(t^{2}-1)\cdot2(t^{2}+t+1)}{(t^{2}+3t+2)(t^{2}-1)^{2}}dt=-\int \frac{t^{2}+t+1}{(t+1)(t+2)}$$
	$$\frac{-2(t^{2}+t+1)}{(t+1)^{2}(t+2)(t-1)}= \frac{A}{t-1} + \frac{B}{t+2} + \frac{C}{t+1} + \frac{D}{(t+1)^{2}}$$
	$$\begin{array} \\
A = -\frac{1}{2} \\
B=2 \\
C = - \frac{3}{2}  \\
D=1

\end{array}$$
$$I(t)= -\frac{1}{2}\ln|t-1| +2\ln|t+2| - \frac{3}{2}\ln|t+1| - \frac{1}{t+1}+C$$
где $t= \frac{\sqrt{ x^{2}-x+1 } - 1}{x}$
