---
tags:
  - calculus
  - integral
links:
  - "[[Понятие неопределённого интеграла. Теорема о структуре множества первообразных]]"
---
$$1. \ \ \int \frac{dx}{(x-a)(x-b)}= \frac{1}{b-a}\ln \bigg|\frac{x-a}{x-b}\bigg | + C$$
$$2. \ \ \int \frac{dx}{x^{2}-a^{2}}=\frac{1}{2a}\ln\bigg| \frac{x-a}{x+a}\bigg|+C$$
$$3.\ \ \int \frac{dx}{x^{2}+a^{2}}=\frac{1}{a}\arctan \frac{x}{a}+C$$
$$4. \ \ \int \frac{dx}{\sin x}=\ln\bigg|\tan \frac{x}{2}\bigg|+C$$
$$5. \ \ \int \frac{dx}{\cos x}=\ln\bigg|\tan\left( \frac{x}{2}+\frac{\pi}{4} \right)\bigg|+C$$
$$6. \ \ \int \frac{dx}{(x^{2}+a^{2})^{2}}= \frac{1}{2a^{2}} \frac{x}{x^{2}+a^{2}}+\frac{1}{2a^{3}}\arctan \frac{x}{a}+C$$
$$7. \ \ \int \frac{dx}{\sqrt{ x^{2}-a^{2} }}=\ln|x+\sqrt{ x^{2}-a^{2} }|+C$$
$$8. \ \ \int \frac{dx}{\sqrt{ a^{2}-x^{2} }}=\arcsin \frac{x}{a}+C$$
$$9. \ \ \int \frac{dx}{\sqrt{ x^{2}+a^{2} }}=\ln|x+\sqrt{ x^{2}+a^{2} }|+C$$
$$10. \ \ \int e^{ a x }\cos b x \ dx= \frac{b\sin bx+a\cos bx}{a^{2}+b^{2}}\cdot e^{ ax }+C$$
$$11. \ \ \int e^{ ax }\sin bx \ dx= \frac{a\sin bx-b\cos bx}{a^{2}+b^{2}}\cdot e^{ ax }+C$$
*Док-во:*
7: $D=\{ x: |x|>|a| \}=D_{1}\cup D_{2} \ \ \ D_{1}=(-\infty,-a), \ D_{2}=(a,+\infty)$
$D_{2}$:
	($\cosh ^{2} x-\sinh ^{2}x=1$) Замена $x=a\cosh t, \ t\in(0,+\infty), \ x\in(a;+\infty)$
	$x^{2}-a^{2}=a^{2}(\cosh ^{2}t-1)=a^{2}\sinh ^{2} t$
	$dx=a\sinh t\ dt$
	$\sinh t>0$
$$I=\int \frac{a\sinh t \ dt}{a|\sinh t|}=\int dt=t+C$$
$$\cosh t=\frac{x}{a}\to \frac{e^{ t }+e^{ -t }}{2}=\frac{x}{a}\to z\cdot e^{ t }>0\to z+\frac{1}{z}=\frac{2x}{a}\to z^{2}-\frac{2x}{a}z+1=0$$
$$z_{1}=\frac{x}{a}+\sqrt{ \frac{x^{2}}{a^{2}}-1 } \ \ z_{2}=\frac{x}{a}-\sqrt{ \frac{x^{2}}{a^{2}}-1 }\to z_{1}\cdot z_{2}=1\to \ln z_{1}+\ln z_{2}=0\to t=\ln z_{1}=$$
$$=\ln \frac{1}{a}(x+\sqrt{ x^{2}-a^{2} })\implies I=\ln \frac{1}{a}(s+\sqrt{ x^{2}-a^{2} })+C=\ln (x+\sqrt{ x^{2}-a^{2} })+\tilde{C}$$
$D_{1}:$ $x<-|a|$ замена $x=-a\cosh t, \ t\in(-\infty ;0), \ x\in(-\infty;-a)$
	$dx=-a\sinh t \ dt$
	$\sinh t<0$
	$$I=\int \frac{-a\sinh t \ dt}{a|\sinh t|}=t+C$$
	$$\cosh t= -\frac{x}{a}\to z=e^{ t }\to z^{2}+\frac{2x}{a}z+1=0 \ \ z_{1}=-\frac{x}{a}-\sqrt{ \frac{x^{2}}{a^{2}} -1}, \ \ z_{2}=-\frac{x}{a} + \sqrt{ \frac{x^{2}}{a^{2}} -1} $
	$$
$$z_{1}\cdot z_{2}=1 \ \ \ln z_{1}+\ln z_{2}=0 \ \ \ln z_{1}<0\to t=\ln\left( -\frac{x}{a}- \sqrt{ \frac{x^{2}}{a^{2}}-1 } \right)=\ln\bigg| \frac{x}{a}+\sqrt{ \frac{x^{2}}{a^{2}}-1 }\to$$
$$I=\ln|x+\sqrt{ x^{2}-a^{2} }|+C$$
6: $I_{2}=\int\frac{dx}{(x^{2}+a^{2})}$
$$\int \frac{dx}{x^{2}+a^{2}}=\bigg |\begin{array} \\
u=\frac{1}{x^{2}+a^{2}} \ \ \ du=- \frac{2x}{(x^{2}+a^{2})^{2}}dx \\
dv=dx \ \ v=x
\end{array}\bigg |= \frac{x}{x^{2}+a^{2}} + 2\int \frac{x^{2}+a^{2}-a^{2}}{(x^{2}+a^{2})^{2}}dx=$$
$$=\frac{x}{x^{2}+a^{2}}+2\int \frac{dx}{x^{2}+a^{2}}-2a^{2}I_{2}\to 2a^{2}I_{2}=\frac{x}{x^{2}+a^{2}}+\int \frac{dx}{x^{2}+a^{2}}=\frac{x}{x^{2}+a^{2}}+\frac{1}{a}\arctan \frac{x}{a}$$
$$\implies I_{2}=\frac{1}{2a^{2}} \frac{x}{x^{2}+a^{2}}+\frac{1}{2a^{3}}\arctan \frac{x}{a}+C$$
10,11: $e^{ (a+bi)x }=e^{ ax }e^{ bxi }=e^{ ax }(\cos bx+i\sin bx)$
$$\int e^{ (a+bi)x }dx=\frac{1}{a+bi}e^{ (a+bi)x }= \frac{a-bi}{a^{2}+b^{2}}(\cos bx+i\sin bx)e^{ ax }$$
$$10: \mathrm{Re}\int e^{ (a+bi)x }dx=\frac{e^{ ax }1}{a^{2}+b^{2}}(a\cos bx+b\sin bx)$$
$$11:\mathrm{Im}\int e^{ (a+bi)x }=e^{ ax }\frac{1}{a^{2}+b^{2}}(a\sin bx-b\cos bx)$$
